Use partial fixpoint

Imp/Stmt/Run.lean
@@ -5,119 +5,88 @@ namespace Imp
 namespace Stmt
 
 /--
-Run a program, with the number of loop iterations limited by the `Nat` parameter. Returns `none`
-if the program doesn't terminate fast enough or if some other problem means the result is undefined
-(e.g. division by zero).
- -/
-def run (σ : Env) (s : Stmt) (n : Nat) : Option Env :=
+Lean allows possibly non-terminating functions if they are in the `Option` monad, so that
+nontermination can be logically modelled as returning `Option.none`. This kind of partial
+function definition needs to be explicitly enabled using `partial_fixpoint`.
+-/
+def run (σ : Env) (s : Stmt) : Option Env :=
   match s with
   | imp {skip;} =>
     some σ
   | imp {~s1 ~s2} => do
-    let σ' ← run σ s1 n
-    run σ' s2 n
+    let σ' ← run σ s1
+    run σ' s2
   | imp {~x := ~e;} => do
     let v ← e.eval σ
     pure (σ.set x v)
   | imp {if (~c) {~s1} else {~s2}} => do
     let v ← c.eval σ
     if v = 0 then
-      run σ s2 n
+      run σ s2
     else
-      run σ s1 n
+      run σ s1
   | imp {while (~c) {~s1}} => do
-    let n + 1 := n
-      | none
     let v ← c.eval σ
     if v = 0 then
       pure σ
     else
-      let σ' ← run σ s1 n
-      run σ' (imp {while (~c) {~s1}}) n
+      let σ' ← run σ s1
+      run σ' (imp {while (~c) {~s1}})
+partial_fixpoint
 
 /-- info: 3628800 -/
 #guard_msgs in
-#eval ((run (Env.init 0 |>.set "n" 10) fact 100).get!.get "out").toNat
+#eval ((run (Env.init 0 |>.set "n" 10) fact).get!.get "out").toNat
 
-example : run σ (imp {skip;}) n = some σ := by
+example : run σ (imp {skip;}) = some σ := by
   simp [run]
 
 /--
-`run` is correct: if it returns an answer, then that final state can be reached by the big-step
-semantics. This is not total correctness - `run` could always return `none` - but it does increase
-confidence.
+`run` is partially correct: if it returns an answer, then that final state can be reached by the
+big-step semantics.
+
+Note that this is not total correctness - `run` could always return `none` and still satisfy this
+theorem.
 -/
-theorem run_some_implies_big_step : run σ s n = some σ' → BigStep σ s σ' := by
-  intro term
-  induction σ, s, n using run.induct generalizing σ' <;> simp_all [run, Option.bind_eq_some_iff]
-  case case2 σ n s1 s2 ih1 ih2 =>
-    let ⟨σ'', run_s1, run_s2⟩ := term
-    -- Right nesting needed to run the first `trivial` before the second `apply_assumption`, which solves a metavariable
-    constructor <;> (apply_assumption <;> trivial)
-  case case3 =>
-    let ⟨v, has_val, next_env⟩ := term
-    subst_eqs
-    constructor <;> trivial
-  case case4 ih1 ih2 =>
-    let ⟨v, has_val, next_env⟩ := term
-    split at next_env
+theorem run_some_implies_big_step : run σ s = some σ' → BigStep σ s σ' := by
+  apply run.partial_correctness
+  intro run ih σ s σ' heq
+  split at heq <;> simp_all
+  · simp [Option.bind_eq_some_iff] at heq
+    obtain ⟨σ'', heq1, heq2⟩ := heq
+    have := ih _ _ _ heq1
+    have := ih _ _ _ heq2
+    constructor <;> assumption
+  · simp [Option.bind_eq_some_iff] at heq
+    obtain ⟨σ'', heq1, heq2⟩ := heq
+    subst heq2
+    constructor <;> assumption
+  · simp [Option.bind_eq_some_iff] at heq
+    obtain ⟨v, heq1, heq2⟩ := heq
+    split at heq2
     · apply BigStep.ifFalse <;> simp_all
     · apply BigStep.ifTrue (v := v) <;> simp_all
-  case case5 ih1 ih2 =>
-    let ⟨v, has_val, next_env⟩ := term
-    split at next_env
-    . simp_all [BigStep.whileFalse]
-    . simp [Option.bind_eq_some_iff] at next_env
-      let ⟨σ'', run_s1_eq, run_while_eq⟩ := next_env
-      apply BigStep.whileTrue (v := v)
-      . simp [*]
-      · assumption
-      . exact ih1 run_s1_eq
-      . exact ih2 _ run_while_eq
+  · simp [Option.bind_eq_some_iff] at heq
+    obtain ⟨v, heq1, heq2⟩ := heq
+    split at heq2
+    · simp at heq2; subst heq2
+      apply BigStep.whileFalse <;> simp_all
+    · simp [Option.bind_eq_some_iff] at heq2
+      obtain ⟨σ'', heq2, heq3⟩ := heq2
+      have := ih _ _ _ heq2
+      have := ih _ _ _ heq3
+      apply BigStep.whileTrue (v := v) <;> assumption
 
-theorem run_some_more_fuel (h : n ≤ m) : run σ s n = some σ' → run σ s m = some σ' := by
-  induction σ, s, n using run.induct generalizing σ' m
-  all_goals simp_all [run, Option.bind_eq_some_iff]
-  case case4 ih1 ih2 =>
-    intro x _
-    split <;> (intro; simp_all)
-  case case5 ih1 ih2 =>
-    cases m
-    case zero => simp at h
-    case succ m =>
-      simp at h
-      simp (config := {contextual:= true}) [run, Option.bind_eq_some_iff]
-      intro x _
-      split
-      · simp
-      · simp [Option.bind_eq_some_iff]
-        intro x s1 s2
-        apply Exists.intro x
-        constructor
-        · apply ih1 h s1
-        · apply ih2 _ h s2
-
-theorem big_step_implies_run_some (h : BigStep σ s σ') : ∃ n, run σ s n = some σ':= by
+/--
+To complete correctness, we prove that if the program has semantics wrt to the big-step-semantics,
+then `run` returns (with the right result).
+-/
+theorem big_step_implies_run_some (h : BigStep σ s σ') : run σ s = some σ':= by
   induction h
-  all_goals try solve | simp_all [run]
-  case «seq» ih1 ih2 =>
-    let ⟨n1, ih1⟩ := ih1
-    let ⟨n2, ih2⟩ := ih2
-    apply Exists.intro (max n1 n2)
-    rw [run]
-    rw [run_some_more_fuel (by omega) ih1]
-    rw [Option.bind_eq_bind, Option.bind_some]
-    rw [run_some_more_fuel (by omega) ih2]
+  all_goals try solve | simp [run, *]
   case «whileTrue» v σ''' body σ' c σ'' hc hnn _ _ ih1 ih2 =>
-    let ⟨n1, ih1⟩ := ih1
-    let ⟨n2, ih2⟩ := ih2
-    apply Exists.intro (max n1 n2 + 1)
-    simp [run, hc]
-    split
-    · contradiction
-    · rw [run_some_more_fuel (by omega) ih1]
-      simp
-      rw [run_some_more_fuel (by omega) ih2]
+    rw [run] -- simp [run] would loop here, so use `rw`
+    simp [*]
   case «whileFalse» h =>
-    apply Exists.intro 1
-    simp [run, h]
+    rw [run]
+    simp [*]
