Imp/Stmt.lean
@@ -6,4 +6,3 @@ import Imp.Stmt.Delab
 import Imp.Stmt.Optimize
 import Imp.Stmt.BigStep
 import Imp.Stmt.Run
-import Imp.Stmt.RunPartial
